computation_prover working. Now can take a user argument to tell it what user functions it should compute on
wrote and proved some functions for modifying reified entailments before sending them to mirror_shard. Changes goals like
!!(A/\B) && C |-- D into
!!A * !!B * C |-- D

reify/denote_tc_assert_b.v
@@ -1,90 +1,13 @@
 Require Import veric.base.
-Require Import veric.expr.
-(*A boolean denote_tc_assert *)
-
-Definition denote_tc_iszero_b v :=
-         match v with Vint i => (Int.eq i Int.zero) 
-                            | Vlong i =>  (Int.eq (Int.repr (Int64.unsigned i)) Int.zero)
-                            | _ => false 
-         end.
-
-Definition denote_tc_nonzero_b v := 
-         match v with Vint i => if negb (Int.eq i Int.zero) then true else false
-                                               | _ => false end.
-
-Definition denote_tc_igt_b i v :=
-     match v with | Vint i1 => (Int.ltu i1 i)
-                     | _ => false
-                  end.
-
-Definition denote_tc_Zge_b z v := 
-          match v with
-                     | Vfloat f => match Float.Zoffloat f with
-                                    | Some n => (Zge_bool z n)
-                                    | None => false
-                                   end
-                     | _ => false 
-                  end.
-
-Definition denote_tc_Zle_b z v := 
-          match v with
-                     | Vfloat f => match Float.Zoffloat f with
-                                    | Some n => (Zle_bool z n)
-                                    | None => false
-                                   end
-                     | _ => false 
-                  end.
-
-Definition denote_tc_samebase_b v1 v2 :=
-                         match v1, v2 with
-                           | Vptr b1 _, Vptr b2 _ => (peq b1 b2)
-                           | _, _ => false 
-                         end.
-
-(** Case for division of int min by -1, which would cause overflow **)
-Definition denote_tc_nodivover_b v1 v2 :=
-match v1, v2 with
-                           | Vint n1, Vint n2 => (negb 
-                                   (Int.eq n1 (Int.repr Int.min_signed) 
-                                    && Int.eq n2 Int.mone))
-                           | _ , _ => false
-                          end.
-
-Require Import msl.msl_standard.
-Require Import veric.base.
-Require Import msl.rmaps.
-Require Import msl.rmaps_lemmas.
 Require Import veric.compcert_rmaps.
-Require Import veric.Clight_lemmas.
-Require Export veric.lift.
-Require Export veric.Cop2.
+Require Import veric.expr.
 
-
-Definition denote_tc_initialized_b id ty rho := 
-match Map.get (te_of rho) id with 
-| Some v => typecheck_val v ty
-| None => false
-end.
-
-Definition isptr_b v := 
-   match v with | Vptr _ _ => true | _ => false end.
-
-Fixpoint denote_tc_assert_b (a: tc_assert) : environ -> bool :=
+Fixpoint denote_tc_assert_b (a: tc_assert) :  bool :=
   match a with
-  | tc_FF _ => `false
-  | tc_noproof => `false
-  | tc_TT => `true
-  | tc_andp' b c => `andb (denote_tc_assert_b b) (denote_tc_assert_b c)
-  | tc_orp' b c => `orb (denote_tc_assert_b b) (denote_tc_assert_b c)
-  | tc_nonzero e => `denote_tc_nonzero_b (eval_expr e)
-  | tc_isptr e => `isptr_b (eval_expr e)
-  | tc_ilt e i => `(denote_tc_igt_b i) (eval_expr e)
-  | tc_Zle e z => `(denote_tc_Zge_b z) (eval_expr e)
-  | tc_Zge e z => `(denote_tc_Zle_b z) (eval_expr e)
-  | tc_samebase e1 e2 => `denote_tc_samebase_b (eval_expr e1) (eval_expr e2)
-  | tc_nodivover v1 v2 => `denote_tc_nodivover_b (eval_expr v1) (eval_expr v2)
-  | tc_initialized id ty => denote_tc_initialized_b id ty
-  | tc_iszero' e => `denote_tc_iszero_b (eval_expr e)
+  | tc_TT => true
+  | tc_andp' b c => andb (denote_tc_assert_b b) (denote_tc_assert_b c)
+  | tc_orp' b c => orb (denote_tc_assert_b b) (denote_tc_assert_b c)
+  | _ => false
  end.
 
 Lemma false_true : False <-> false=true.
@@ -133,26 +56,7 @@ Tactic Notation "bool_r" "in" "*" :=
 bool_s.
 
 Definition denote_te_assert_b_eq : forall a rho, 
-denote_tc_assert a rho <-> is_true (denote_tc_assert_b a rho).
-Proof. intros. split; intros.
-induction a; simpl in *; super_unfold_lift; bool_r in *; intuition;
-simpl in *;
-try destruct (eval_expr e); simpl in *;
-try match goal with 
-| [ H : if ?e then True else False |- _ ] => destruct e; simpl; inv H
-| [ H : match ?e with | _ => _  end |- _ ] => destruct e; simpl in *; inv H
-end; auto; try congruence;
-unfold denote_tc_initialized, denote_tc_initialized_b in *;
-destruct H. destruct H. rewrite H. auto.
-
-induction a; simpl in *; super_unfold_lift; bool_r in *; intuition; try congruence;
-simpl in *;
-try destruct (eval_expr e); simpl in *; try congruence;
-try match goal with 
-| [ H : (if ?e then true else false) = true |- _ ] => destruct e; simpl; inv H
-| [ H : (match ?e with | _ => _ end) = true |- _ ] => destruct e; simpl in *; inv H
-end; auto; try congruence.
-unfold denote_tc_initialized, denote_tc_initialized_b in *.
-destruct (Map.get (te_of rho) e). exists v. auto.
-congruence.
+is_true (denote_tc_assert_b a) -> denote_tc_assert a rho.
+Proof. intros. induction a; inv H; simpl; unfold_lift; simpl; auto;
+bool_r in *; intuition.
 Qed.
