reify/preproc.v
@@ -1,0 +1,420 @@
+Require Import floyd.proofauto.
+Require Import mirror_cancel.
+
+Local Open Scope logic.
+
+
+Fixpoint flatten_top_conjuncts {types} p : Expr.exprs types :=
+match p with
+| Func 5%nat (a :: b :: nil) => flatten_top_conjuncts a ++ flatten_top_conjuncts b
+| _ => p::nil
+end.
+
+Definition reflect_and {T} a b := @Func T 5%nat (a :: b :: nil).
+
+Fixpoint unflatten_conjuncts {types} l : Expr.expr types :=
+match l with
+| nil => Func (functions.True_f nil) nil
+| h::nil => h
+| h::t => Func 5%nat (h::(unflatten_conjuncts t)::nil)
+end .
+
+Fixpoint unflatten_conjuncts_sep {types} l : Sep.sexpr types :=
+match l with
+| nil => Sep.Inj (Func (functions.True_f nil) nil)
+| h::nil => Sep.Inj h
+| h::t => Sep.Star (Sep.Inj h) (unflatten_conjuncts_sep t)
+end .
+
+Definition lift_and {types} e : Sep.sexpr types :=
+unflatten_conjuncts_sep (flatten_top_conjuncts e).
+
+Fixpoint lift_ands {types} s : Sep.sexpr types :=
+match s with
+| Sep.Star a b => Sep.Star (lift_ands a) (lift_ands b)
+| Sep.Inj e => lift_and e
+| _ => s
+end.
+
+Definition is_true_e {t} (p: Expr.expr t) :=
+match p with
+| Func f nil  => beq_nat (functions.True_f nil) f
+| _ => false
+end.
+
+
+Definition not_true {t} (p: Expr.expr t) := negb (is_true_e p).
+
+Definition remove_true {t} l :=
+filter (@not_true t) l.
+
+Definition remove_trues {t} (e : Expr.expr t) :=
+unflatten_conjuncts (remove_true (flatten_top_conjuncts e)).
+
+Lemma provable_l : forall t l f uenv ,
+nth_error f 5 = Some (functions.and_signature t) ->
+Provable f uenv nil (Func 5%nat l) ->
+exists a, exists b, l = a::b::nil.
+Proof.
+intros. unfold Provable in H0. simpl in *; rewrite H in *; simpl in *.
+destruct l; simpl in H0; intuition.
+destruct l; simpl in H0; intuition.
+destruct (exprD f uenv nil e tvProp); intuition.
+destruct l. eauto.
+destruct (exprD f uenv nil e tvProp); intuition.
+destruct (exprD f uenv nil e0 tvProp); intuition.
+Qed.
+
+Lemma Provable_reflect_and : forall t a b uenv f,
+ nth_error f 5 = Some (functions.and_signature t) -> 
+(Provable f uenv nil (reflect_and a b) <-> Provable f uenv nil a /\ Provable f uenv nil b).
+Proof.
+intros; split; intros; unfold Provable in *;
+simpl in *; try rewrite H in *; simpl in *;
+destruct (exprD f uenv nil a tvProp); destruct (exprD f uenv nil b tvProp); intuition. 
+Qed.
+
+Lemma Provable_f5_and : forall t a b uenv f,
+ nth_error f 5 = Some (functions.and_signature t) -> 
+(Provable f uenv nil
+         (Func 5%nat (a :: b :: nil)) <->  Provable f uenv nil a /\ Provable f uenv nil b).
+Proof.
+intros. assert (Z := Provable_reflect_and). unfold reflect_and in *. apply Z; auto.
+Qed.
+
+Hint Rewrite Provable_reflect_and Provable_f5_and using auto: Provable_and.
+
+Ltac rp := autorewrite with Provable_and in *.
+
+Lemma remove_true_app : forall {t} x x0,
+@remove_true t (x ++ x0) =
+remove_true x ++ remove_true x0.
+Proof.
+intros. unfold remove_true. revert x0.
+induction x; intros; auto.
+simpl. if_tac. rewrite <- app_comm_cons. f_equal. auto.
+auto.
+Qed.
+
+Lemma provable_unflatten_cons : forall t l a f uenv,
+                                  nth_error f 5 = Some (functions.and_signature t) ->
+                                  nth_error f (functions.True_f nil) = Some (functions.True_signature t) ->
+                                  (Provable f uenv nil (unflatten_conjuncts (a :: l)) <->
+                                  Provable f uenv nil a /\ Provable f uenv nil (unflatten_conjuncts l)).
+Proof.
+intros; split; intros;
+induction l; auto. simpl. unfold Provable in *; simpl in *; rewrite H0; auto; clear H0.
+intuition.
+simpl; auto.
+simpl in H1; rp; intuition.
+intuition.
+simpl; rp; intuition.
+Qed.
+
+Hint Rewrite provable_unflatten_cons: Provable_and.
+
+Lemma unflatten_conjuncts_app :
+forall t l1 l2 f uenv, 
+nth_error f 5%nat = Some (functions.and_signature t) -> 
+nth_error f (functions.True_f nil) = Some (functions.True_signature t) ->
+(Provable f uenv nil
+(Func 5%nat 
+((unflatten_conjuncts l1) :: ((unflatten_conjuncts) l2) :: nil)) <->
+Provable f uenv nil
+(unflatten_conjuncts (l1 ++ l2))).
+Proof.
+intros; split; intros.
+  + generalize dependent l2. induction l1; intros. 
+      - simpl. simpl in H1. 
+        unfold Provable in *; simpl in *; try rewrite H in *; try rewrite H0 in *; clear H0;
+        simpl in *. 
+        destruct (exprD f uenv nil (unflatten_conjuncts l2) tvProp);
+          intuition.
+      - rewrite <- app_comm_cons. rp; intuition.
+        apply IHl1. rp; auto.
+  + induction l1; auto.
+      - rp; intuition. simpl. unfold Provable; simpl; simpl in H0; rewrite H0; simpl; auto.
+      - rewrite <- app_comm_cons in *.
+        rp. intuition. auto. auto.
+        auto. auto.
+Qed.
+
+Lemma provable_l_remove : forall t l f uenv,
+nth_error f 5 = Some (functions.and_signature t) ->
+Provable f uenv nil (remove_trues (Func 5%nat l)) ->
+exists a, exists b, l = a::b::nil.
+Proof.
+intros. unfold Provable in H0.
+destruct l; simpl in *; try rewrite H in *; intuition.
+destruct l; simpl in *; try rewrite H in *; intuition.
+simpl in *.
+destruct (exprD f uenv nil e tvProp); intuition.
+destruct l; eauto.
+simpl in H0. rewrite H in H0. simpl in H0.
+destruct (exprD f uenv nil e tvProp); intuition.
+destruct (exprD f uenv nil e0 tvProp); intuition.
+Qed.
+
+Lemma func_True : forall t f uenv,  
+nth_error f (functions.True_f nil) = Some (functions.True_signature t) ->
+Provable f uenv nil (Func (functions.True_f nil) nil) = True.
+Proof.
+intros.
+unfold Provable.
+simpl in *;  rewrite H; simpl; auto.
+Qed.
+
+Hint Rewrite func_True: Provable_and.
+
+
+Lemma Provable_remove_trues : forall t e uenv f,
+nth_error f 5 = Some (functions.and_signature t) ->
+nth_error f (functions.True_f nil) = Some (functions.True_signature t) ->
+(Provable f uenv nil e <-> Provable f uenv nil (remove_trues e)). 
+Proof.
+intros; split; induction e; intros; auto.
+(* + unfold remove_trues. unfold flatten_top_conjuncts.
+   unfold remove_true. unfold filter. simpl. unfold not_true. 
+   destruct (is_true_e (Const t0)). simpl. unfold Provable; simpl; auto.
+   apply H0.*)
+ + do 5 (destruct f0; [ unfold remove_trues; try destruct l; auto | ]). 
+   destruct f0.
+   assert (L := provable_l _ _ _ _ H H2).
+   destruct L. destruct H3. subst.
+   unfold remove_trues. simpl.
+   rewrite remove_true_app.
+   rewrite <-unflatten_conjuncts_app.
+   rp. destruct H2. 
+   rewrite Forall_forall in H1. unfold remove_trues in H1.
+   intuition.
+   auto. auto.
+   do 43 (destruct f0; [ unfold remove_trues; try destruct l; auto | auto ]).
+   unfold Provable; simpl. auto.
+   destruct l; auto.
+ + do 5 (destruct f0; [ unfold remove_trues; try destruct l; auto | ]). 
+   destruct f0.
+   assert (L := provable_l_remove _ _ _ _ H H2).
+   destruct L. destruct H3. subst.
+   unfold remove_trues in H2. simpl in H2.
+   rewrite remove_true_app in H2. rewrite <- unflatten_conjuncts_app in H2.
+   rp. rewrite Forall_forall in H1. 
+   intuition.
+   auto. auto.
+   
+   do 43 (destruct f0; [ unfold remove_trues; try destruct l; auto | auto ]).
+   unfold remove_trues in *. simpl in H2. destruct l; auto.
+Qed.
+
+Lemma unflatten_conjuncts_sep_app : forall t f p uenv l1 l2,
+nth_error f (functions.True_f nil) = Some (functions.True_signature t) ->
+Sep.sexprD f p uenv nil 
+(Sep.Star (unflatten_conjuncts_sep l1) (unflatten_conjuncts_sep l2)) =
+Sep.sexprD f p uenv nil
+         (unflatten_conjuncts_sep
+            (l1 ++ l2)).
+Proof.
+intros. apply pred_ext.
+induction l1. simpl (unflatten_conjuncts_sep nil).
+Opaque functions.True_f.
+simpl. rewrite H. simpl. 
+unfold_VericSepLogic. entailer. 
+simpl in *. remember (l1 ++ l2).
+destruct l. simpl. destruct l1; inv Heql.
+simpl. destruct (exprD f uenv nil a tvProp).
+unfold_VericSepLogic. entailer. destruct l2; inv H0; simpl; entailer.
+simpl in *. rewrite H in *. simpl in *.
+unfold VericSepLogic.inj in *. 
+unfold VericSepLogic.star in *.
+unfold VericSepLogic_Kernel.emp in *.
+entailer!.
+unfold VericSepLogic.inj in *. 
+unfold VericSepLogic.star in *.
+unfold VericSepLogic_Kernel.emp in *. unfold BadInj.
+entailer!. simpl.
+destruct l1. simpl. destruct (exprD f uenv nil a tvProp).
+simpl in IHl1. rewrite H in *. simpl in *.
+unfold VericSepLogic.inj in *. 
+unfold VericSepLogic.star in *.
+unfold VericSepLogic_Kernel.emp in *.
+entailer. 
+unfold VericSepLogic.inj in *. 
+unfold VericSepLogic.star in *.
+unfold VericSepLogic_Kernel.emp in *.
+entailer.
+inv Heql. simpl.
+destruct ( exprD f uenv nil a tvProp).
+simpl in IHl1. entailer!.
+unfold VericSepLogic.star in *.
+cancel.
+apply IHl1.
+simpl in *. entailer. unfold BadInj. entailer!.
+unfold VericSepLogic.star in *.
+cancel.
+apply IHl1.
+
+induction l1; auto.
+  + simpl. rewrite H.
+    simpl. unfold VericSepLogic.inj. entailer!. 
+  + simpl in *.
+    remember (l1 ++ l2). destruct (l). 
+      - simpl in *.
+        rewrite H in *. simpl in *.
+        destruct l1; inv Heql. simpl.
+        destruct (exprD f uenv nil a tvProp); [ | unfold BadInj, VericSepLogic.inj; entailer].
+        unfold VericSepLogic.inj in *. 
+        unfold VericSepLogic.star in *.
+        unfold VericSepLogic_Kernel.emp in *.
+        entailer. simpl in IHl1. rewrite H in *. simpl in IHl1.
+        unfold VericSepLogic.inj in *. 
+        unfold VericSepLogic.star in *.
+        unfold VericSepLogic_Kernel.emp in *.
+        entailer. 
+        autorewrite with norm in IHl1. auto.
+        apply Cveric.
+      - simpl in *.
+        destruct l1; inv Heql.
+          * simpl. destruct (exprD f uenv nil a tvProp); 
+                   [ | unfold BadInj, VericSepLogic.inj; entailer].
+            simpl in *. rewrite H in *. simpl in *. destruct l. simpl in *.
+            destruct (exprD f uenv nil e tvProp);
+                     [ | unfold BadInj, VericSepLogic.inj; entailer].
+            unfold VericSepLogic.inj in *. 
+            unfold VericSepLogic.star in *.
+            unfold VericSepLogic_Kernel.emp in *.
+            entailer. autorewrite with norm in IHl1; [ | apply Cveric].
+            auto.
+            simpl in *.
+            destruct (exprD f uenv nil e tvProp); 
+                   [ | unfold BadInj, VericSepLogic.inj; entailer].
+            unfold VericSepLogic.inj in *. 
+            unfold VericSepLogic.star in *.
+            unfold VericSepLogic_Kernel.emp in *.
+            entailer.
+            unfold VericSepLogic.inj in *. 
+            unfold VericSepLogic.star in *.
+            unfold VericSepLogic_Kernel.emp in *.
+            cancel.
+            autorewrite with norm in *. auto.
+            apply Cveric.
+            unfold VericSepLogic.inj in *. 
+            unfold VericSepLogic.star in *.
+            unfold VericSepLogic_Kernel.emp in *.
+            entailer.
+          * simpl in *.
+            unfold VericSepLogic.inj in *. 
+            unfold VericSepLogic.star in *.
+            unfold VericSepLogic_Kernel.emp in *.
+            destruct (exprD f uenv nil a tvProp); entailer.
+Qed.
+
+Lemma Provable_lift_and : forall t e uenv f p,
+nth_error f 5 = Some (functions.and_signature t) ->
+nth_error f (functions.True_f nil) = Some (functions.True_signature t) ->
+Sep.sexprD f p uenv nil (Sep.Inj e) = Sep.sexprD f p uenv nil (lift_and e).
+Proof.
+intros. apply pred_ext.
+  + simpl. 
+    induction e; auto.
+    do 6 (destruct f0; auto).
+    simpl. simpl in H. rewrite H. simpl.
+    destruct l; simpl. 
+      - unfold BadInj.
+        unfold VericSepLogic.inj. apply derives_extract_prop.
+        contradiction.
+      - destruct l. simpl. rewrite H. simpl.
+        destruct (exprD f uenv nil e tvProp). auto.
+        auto.
+        destruct l. 
+          * rewrite Forall_forall in *.
+            assert (Ee := (H1 e)). simpl in Ee. intuition. clear H2 H5.
+            assert (Ee0 := (H1 e0)). simpl in Ee0. intuition. clear H2 H6.
+            destruct (exprD f uenv nil e tvProp).
+            simpl.
+            destruct (exprD f uenv nil e0 tvProp). 
+            unfold VericSepLogic.inj in *. unfold VericSepLogic_Kernel.emp in *.
+            unfold lift_and. simpl.
+            rewrite <- unflatten_conjuncts_sep_app.
+            simpl. entailer. autorewrite with norm in *.
+            eapply derives_trans.
+            instantiate (1:= emp * emp). cancel.
+            unfold VericSepLogic.star. 
+            apply sepcon_derives; auto. auto.
+
+            unfold BadInj. simpl. unfold VericSepLogic.inj.  entailer!.
+            unfold BadInj. simpl. unfold VericSepLogic.inj. entailer!.
+          * simpl in *. rewrite H in *. simpl in *. cancel.
+  + induction e; auto.
+
+do 6 (destruct f0; auto).
+simpl. simpl in H. rewrite H. simpl.
+destruct l; simpl. rewrite H. simpl.
+unfold BadInj. entailer.
+destruct l. simpl. rewrite H. simpl.
+destruct (exprD f uenv nil e tvProp). auto.
+auto.
+destruct l. 
+rewrite Forall_forall in *.
+assert (Ee := (H1 e)). simpl in Ee. intuition. clear H2 H5.
+assert (Ee0 := (H1 e0)). simpl in Ee0. intuition. clear H2 H6.
+unfold lift_and. simpl.
+rewrite <- unflatten_conjuncts_sep_app.
+simpl. unfold VericSepLogic.star.
+destruct (exprD f uenv nil e tvProp).
+simpl.
+destruct (exprD f uenv nil e0 tvProp). 
+unfold VericSepLogic.inj in *. unfold VericSepLogic_Kernel.emp in *.
+simpl. 
+unfold VericSepLogic.star. 
+eapply derives_trans.
+Focus 2.
+instantiate (1:= ((!!t0 && emp) * (!!t1 && emp))). entailer!. 
+apply sepcon_derives; auto. 
+
+unfold BadInj in *. unfold VericSepLogic.inj in *.
+eapply derives_trans. 
+apply sepcon_derives. apply H4. apply H3.
+entailer!.
+
+unfold BadInj.
+eapply derives_trans.
+apply sepcon_derives; eassumption.
+unfold VericSepLogic.inj, BadInj.
+destruct (exprD f uenv nil e0 tvProp); entailer!. 
+auto.
+
+simpl in *. rewrite H in *. simpl in *.
+cancel.
+
+Qed.
+
+Lemma lift_ands_eq : forall t f p s uenv,
+nth_error f 5 = Some (functions.and_signature t) ->
+nth_error f (functions.True_f nil) = Some (functions.True_signature t) ->
+Sep.sexprD f p uenv nil s =
+Sep.sexprD f p uenv nil (lift_ands s).
+Proof.
+intros.
+apply pred_ext.
++ induction s; auto.
+    - simpl. rewrite <- Provable_lift_and; auto.
+    - simpl. unfold VericSepLogic.star. apply sepcon_derives; auto.
++ induction s; auto.
+    - simpl. rewrite <- Provable_lift_and; auto.
+    - simpl. unfold VericSepLogic.star. apply sepcon_derives; auto.
+Qed.  
+  
+Lemma goal_lift_and :
+forall t f preds uenv a l r,
+nth_error f 5 = Some (functions.and_signature t) ->
+nth_error f (functions.True_f nil) = Some (functions.True_signature t) ->
+(goalD (functions.all_types_r t) f preds uenv nil (a, (l,r)) <-> 
+goalD (functions.all_types_r t) f preds uenv nil (a, ((lift_ands l), (lift_ands r)))).
+intuition.
+ + induction a. 
+     - simpl in *. 
+       repeat rewrite <- lift_ands_eq; auto.
+     - simpl. intros. simpl in *. destruct a0; intuition.
+ + induction a.
+     - simpl in *. do 2 rewrite <- lift_ands_eq in *; auto.
+     - simpl in *. destruct a0; intuition.
+Qed.
